theories/typing/cont.v
@@ -13,7 +13,7 @@ Section typing.
     tctx_incl E L T (T' (list_to_vec args)) →
     typed_body E L C T (k (of_val <$> args)).
   Proof.
-    iIntros (HC Hincl) "!#". iIntros (tid qE) "#HEAP #LFT Htl HE HL HC HT".
+    iIntros (HC Hincl) "!#". iIntros (tid qE) "#LFT Htl HE HL HC HT".
     iMod (Hincl with "LFT HE HL HT") as "(HE & HL & HT)".
     iSpecialize ("HC" with "HE []"); first done.
     rewrite -{3}(vec_to_list_of_list args). iApply ("HC" with "Htl HL HT").
@@ -26,15 +26,15 @@ Section typing.
        typed_body E L1 (k ◁cont(L1, T') :: C) (T' args) (subst_v (kb::argsb) (k:::args) econt)) →
     typed_body E L2 C T (e2 cont: kb argsb := econt).
   Proof.
-    iIntros (Hc1 Hc2 He2 Hecont) "!#". iIntros (tid qE) "#HEAP #LFT Htl HE HL HC HT". iApply wp_let'.
+    iIntros (Hc1 Hc2 He2 Hecont) "!#". iIntros (tid qE) "#LFT Htl HE HL HC HT". iApply wp_let'.
     { simpl. rewrite decide_left. done. }
-    iModIntro. iApply (He2 with "HEAP LFT Htl HE HL [HC] HT"). clear He2.
+    iModIntro. iApply (He2 with "LFT Htl HE HL [HC] HT"). clear He2.
     iIntros "HE". iLöb as "IH". iIntros (x) "H".
     iDestruct "H" as %[->|?]%elem_of_cons; last by iApply ("HC" with "HE").
     iIntros (args) "Htl HL HT". iApply wp_rec; try done.
     { rewrite Forall_fmap Forall_forall=>? _. rewrite /= to_of_val. eauto. }
     { by rewrite -(subst_v_eq (_ :: _) (RecV _ _ _ ::: _)). }
-    iNext. iApply (Hecont with "HEAP LFT Htl HE HL [HC] HT").
+    iNext. iApply (Hecont with "LFT Htl HE HL [HC] HT").
     by iApply "IH".
   Qed.
 End typing.
