theories/typing/int.v
@@ -25,7 +25,7 @@ Section typing.
   Lemma type_int_instr (z : Z) E L :
     typed_instruction_ty E L [] #z int.
   Proof.
-    iAlways. iIntros (tid qE) "_ _ $ $ $ _". wp_value.
+    iAlways. iIntros (tid qE) "_ $ $ $ _". wp_value.
     by rewrite tctx_interp_singleton tctx_hasty_val.
   Qed.
 
@@ -40,7 +40,7 @@ Section typing.
   Lemma type_plus_instr E L p1 p2 :
     typed_instruction_ty E L [p1 ◁ int; p2 ◁ int] (p1 + p2) int.
   Proof.
-    iAlways. iIntros (tid qE) "_ _ $ $ $". rewrite tctx_interp_cons tctx_interp_singleton.
+    iAlways. iIntros (tid qE) "_ $ $ $". rewrite tctx_interp_cons tctx_interp_singleton.
     iIntros "[Hp1 Hp2]".
     wp_bind p1. iApply (wp_hasty with "Hp1").
     iIntros ([[]|]) "_ H1"; try iDestruct "H1" as "[]".
@@ -61,7 +61,7 @@ Section typing.
   Lemma type_minus_instr E L p1 p2 :
     typed_instruction_ty E L [p1 ◁ int; p2 ◁ int] (p1 - p2) int.
   Proof.
-    iAlways. iIntros (tid qE) "_ _ $ $ $". rewrite tctx_interp_cons tctx_interp_singleton.
+    iAlways. iIntros (tid qE) "_ $ $ $". rewrite tctx_interp_cons tctx_interp_singleton.
     iIntros "[Hp1 Hp2]".
     wp_bind p1. iApply (wp_hasty with "Hp1").
     iIntros ([[]|]) "_ H1"; try iDestruct "H1" as "[]".
@@ -82,7 +82,7 @@ Section typing.
   Lemma type_le_instr E L p1 p2 :
     typed_instruction_ty E L [p1 ◁ int; p2 ◁ int] (p1 ≤ p2) bool.
   Proof.
-    iAlways. iIntros (tid qE) "_ _ $ $ $". rewrite tctx_interp_cons tctx_interp_singleton.
+    iAlways. iIntros (tid qE) "_ $ $ $". rewrite tctx_interp_cons tctx_interp_singleton.
     iIntros "[Hp1 Hp2]".
     wp_bind p1. iApply (wp_hasty with "Hp1").
     iIntros ([[]|]) "_ H1"; try iDestruct "H1" as "[]".
