theories/typing/own.v
@@ -197,8 +197,8 @@ Section typing.
     let n' := Z.to_nat n in
     typed_instruction_ty E L [] (new [ #n ]%E) (own_ptr n' (uninit n')).
   Proof.
-    intros. iAlways. iIntros (tid q) "#HEAP #LFT $ $ $ _".
-    iApply (wp_new with "HEAP"); try done. iModIntro.
+    intros. iAlways. iIntros (tid q) "#LFT $ $ $ _".
+    iApply wp_new; first done. iModIntro.
     iIntros (l vl) "(% & H† & Hlft)". subst. rewrite tctx_interp_singleton tctx_hasty_val.
     iNext. rewrite freeable_sz_full Z2Nat.id //. iFrame.
     iExists vl. iFrame. by rewrite Nat2Z.id uninit_own.
@@ -231,7 +231,7 @@ Section typing.
     Z.of_nat (ty.(ty_size)) = n →
     typed_instruction E L [p ◁ box ty] (delete [ #n; p])%E (λ _, []).
   Proof.
-    iIntros (<-) "!#". iIntros (tid eq) "#HEAP #LFT $ $ $ Hp". rewrite tctx_interp_singleton.
+    iIntros (<-) "!#". iIntros (tid eq) "#LFT $ $ $ Hp". rewrite tctx_interp_singleton.
     wp_bind p. iApply (wp_hasty with "Hp"). iIntros ([[]|]) "_ Hown";
       try iDestruct "Hown" as "[]". iDestruct "Hown" as "[H↦∗: >H†]".
     iDestruct "H↦∗:" as (vl) "[>H↦ Hown]". rewrite tctx_interp_nil.
